LeanVerus/trans/soundness.lean
@@ -5,26 +5,34 @@ import LeanVerus.Sst.Domain
 import LeanVerus.Sst.Exp_Rep
 import LeanVerus.Air_ast.«Air-ast»
 import LeanVerus.Trans.Trans
+import LeanVerus.Trans.Axioms
 
 open sst typing MSFirstOrder MSLanguage AirSorts airFunc BoundedFormula
 
 
 -- The sorted carrier (AirSorts → Type) of an AirMod model.
 abbrev AirMod.toFam (P T F : Type) [AirMod P T F] : AirSorts → Type := AirCarrier P T F
-
+abbrev AirMod.toFam' (P T F : Type) : AirSorts → Type := AirCarrier P T F
 variable (tenv : typ_env) (dom_aux : ClosedTyp → Type)
+
+lemma trans_sort_correspondence {Γ : context} {t : Typ}
+  (e₁ e₂ : sst.Exp)
+  (hty₁ : Γ ⊢ e₁ : t) (hty₂ : Γ ⊢ e₂ : t):
+  (trans_exp e₁ preludeAxioms).1.1 = (trans_exp e₂ preludeAxioms).1.1 := sorry
+
+-- TODO: define a toy example
+
 
 theorem trans_sound
   {Γ : context} {t : Typ} {dom_aux : ClosedTyp → Type}
   (e₁ e₂ : sst.Exp)
   (hty₁ : Γ ⊢ e₁ : t) (hty₂ : Γ ⊢ e₂ : t)
-  -- the two translations land in the same sort
-  (h_sort : (trans_exp e₁ ∅).1.1 = (trans_exp e₂ ∅).1.1)
   -- in every AIR model satisfying the generated axioms, the translations evaluate equally
   (h_air : ∀ (P T F : Type) [AirMod P T F],
-    AirMod.toFam P T F ⊨ (trans_exp e₁ ∅).2 ∪ (trans_exp e₂ ∅).2 →
+    AirMod.toFam P T F ⊨ (trans_exp e₁ preludeAxioms).2 ∪ (trans_exp e₂ preludeAxioms).2 →
     ∀ (v : TransVarFam →ₛ AirMod.toFam P T F),
-      ((trans_exp e₁ ∅).1.2.equal (h_sort ▸ (trans_exp e₂ ∅).1.2)).Realize v) :
+      ((trans_exp e₁ preludeAxioms).1.2.equal ((trans_sort_correspondence e₁ e₂ hty₁ hty₂) ▸ (trans_exp e₂ preludeAxioms).1.2)).Realize v) :
   -- [e₁] = [e₂]: the SST denotations agree for all variable environments
   ∀ (venv : val_vars tenv Γ dom_aux),
+    -- TODO: some relations between v and venv
     exp_rep dom_aux Γ tenv venv t e₁ hty₁ = exp_rep dom_aux Γ tenv venv t e₂ hty₂ := sorry
